

# CS 30: Recursive Functions Practice

Find the generalized pattern for each of the following:

1.

$n$	$f(n)$	$f(1) = 1$ $f(2) = 4 = 1 + 3 = 1 + (2 + 1)$ $f(3) = 8 = 4 + 4 = 4 + (3 + 1)$ $f(4) = 13 = 8 + 5 = 8 + (4 + 1)$ $f(5) = 19 = 13 + 6 = 13 + (5 + 1)$ $f(6) = 26 = 19 + 7 = 19 + (6 + 1)$  $f(n) = f(n - 1) + (n + 1)$ when $n \geq 2$
1	1	
2	4	
3	8	
4	13	
5	19	
6	26	

2.

$n$	$f(n)$	$f(1) = 5 = 5 + 0$ $f(2) = 7 = 5 + 2$ $f(3) = 9 = 7 + 2$ $f(4) = 11 = 9 + 2$ $f(5) = 13 = 11 + 2$ $f(6) = 15 = 13 + 2$  $f(n) = 5 + 2(n - 1) = 5 + 2n - 2 = 2n + 3$  For more information: <a href="https://youtu.be/_cooC3yG_p0">https://youtu.be/_cooC3yG_p0</a>
1	5	
2	7	
3	9	
4	11	
5	13	
6	15	

3.

$n$	$f(n)$	$f(1) = 2 = 2^1$ $f(2) = 4 = 2^2$ $f(3) = 8 = 2^3$  $f(n) = 2^n$
1	2	
2	4	
3	8	
4	16	
5	32	
6	64	

4.

$n$	$f(n)$	$f(1) = 1$ $f(2) = 2 = 2 \cdot 1$ $f(3) = 6 = 3 \cdot 2$ $f(4) = 24 = 6 \cdot 4$ $f(5) = 120 = 24 \cdot 5$ $f(6) = 720 = 120 \cdot 6$  $f(n) = f(n - 1) \cdot n$ when $n \geq 2$
1	1	
2	2	
3	6	
4	24	
5	120	
6	720	

5.

$n$	$f(n)$	$f(1) = 2$ $f(2) = 3$ $f(3) = 6 = 2 \cdot 3$ $f(4) = 18 = 3 \cdot 6$ $f(5) = 108 = 6 \cdot 18$ $f(6) = 1944 = 18 \cdot 108$  $f(n) = f(n - 1) \cdot f(n - 2)$ when $n > 2$
1	2	
2	3	
3	6	
4	18	
5	108	
6	1944	